@prefix owl:   <http://www.w3.org/2002/07/owl#> .
@prefix rdf:   <http://www.w3.org/1999/02/22-rdf-syntax-ns#> .
@prefix rdfs:  <http://www.w3.org/2000/01/rdf-schema#> .
@prefix xsd:   <http://www.w3.org/2001/XMLSchema#> .
@prefix IMMoRTALS: <http://securboration.com/immortals/ontology/r1.0.0#> .
@prefix IMMoRTALS_bytecode: <http://securboration.com/immortals/ontology/r1.0.0/bytecode#> .
@prefix IMMoRTALS_condition: <http://securboration.com/immortals/ontology/r1.0.0/condition#> .
@prefix IMMoRTALS_core: <http://securboration.com/immortals/ontology/r1.0.0/core#> .
@prefix IMMoRTALS_dfu: <http://securboration.com/immortals/ontology/r1.0.0/dfu#> .
@prefix IMMoRTALS_functionality_datatype: <http://securboration.com/immortals/ontology/r1.0.0/functionality/datatype#> .
@prefix IMMoRTALS_resources: <http://securboration.com/immortals/ontology/r1.0.0/resources#> .
@prefix IMMoRTALS_resources_compute: <http://securboration.com/immortals/ontology/r1.0.0/resources/compute#> .
@prefix IMMoRTALS_resources_constraints: <http://securboration.com/immortals/ontology/r1.0.0/resources/constraints#> .
@prefix IMMoRTALS_resources_environment: <http://securboration.com/immortals/ontology/r1.0.0/resources/environment#> .
@prefix IMMoRTALS_functionality: <http://securboration.com/immortals/ontology/r1.0.0/functionality#> .
@prefix IMMoRTALS_resources_gps: <http://securboration.com/immortals/ontology/r1.0.0/resources/gps#> .
@prefix IMMoRTALS_resources_logical: <http://securboration.com/immortals/ontology/r1.0.0/resources/logical#> .
@prefix IMMoRTALS_resources_memory: <http://securboration.com/immortals/ontology/r1.0.0/resources/memory#> .
@prefix IMMoRTALS_resources_network: <http://securboration.com/immortals/ontology/r1.0.0/resources/network#> .
@prefix IMMoRTALS_resources_performance: <http://securboration.com/immortals/ontology/r1.0.0/resources/performance#> .
@prefix IMMoRTALS_resources_performance_ResourcePerformanceType: <http://securboration.com/immortals/ontology/r1.0.0/resources/performance/ResourcePerformanceType#> .
@prefix IMMoRTALS_resources_perturbation: <http://securboration.com/immortals/ontology/r1.0.0/resources/perturbation#> .
@prefix IMMoRTALS_condition_ConditionSensitivityImpactType: <http://securboration.com/immortals/ontology/r1.0.0/condition/ConditionSensitivityImpactType#> .
@prefix IMMoRTALS_resources_constraints_OperatorType: <http://securboration.com/immortals/ontology/r1.0.0/resources/constraints/OperatorType#> .
@prefix IMMoRTALS_resources_logical_OsType: <http://securboration.com/immortals/ontology/r1.0.0/resources/logical/OsType#> .
@prefix IMMoRTALS_resources_memory_MemoryType: <http://securboration.com/immortals/ontology/r1.0.0/resources/memory/MemoryType#> .
@prefix IMMoRTALS_java_lang: <http://securboration.com/immortals/ontology/r1.0.0/java/lang#> .

<http://securboration.com/immortals/ontology/r1.0.0>
        a                owl:Ontology ;
        rdfs:comment     "Automatically generated by the POJO-to-triples Maven plugin, Securboration Inc." ;
        owl:versionInfo  "r1.0.0" .

IMMoRTALS_resources_constraints:Variable
        a             owl:Class ;
        rdfs:comment  " A variable for use in an expression \n@author jstaples\n@creationTimestamp 2016.02.08 at 15:05:31 EST" .

IMMoRTALS:has_localDevice
        a             owl:ObjectProperty ;
        rdfs:comment  " The local device\n@creationTimestamp 2016.02.08 at 15:11:46 EST" ;
        rdfs:domain   IMMoRTALS_resources_network:NetworkConnection ;
        rdfs:range    IMMoRTALS_resources:ExecutionPlatform .

IMMoRTALS_condition:LibraryUnavailable
        a                owl:Class ;
        rdfs:comment     " A condition where some library is unavailable \n@author jstaples\n@creationTimestamp 2016.02.08 at 14:45:34 EST" ;
        rdfs:subClassOf  IMMoRTALS_condition:PlatformCondition .

IMMoRTALS:has_restoreState
        a             owl:ObjectProperty ;
        rdfs:comment  " A DFU that allows us to set the state before context switching\n@creationTimestamp 2016.02.08 at 14:49:12 EST" ;
        rdfs:domain   IMMoRTALS_dfu:ContextSwitchingMechanism ;
        rdfs:range    IMMoRTALS_dfu:Dfu .

IMMoRTALS_java_lang:Object
        a       owl:Class .

IMMoRTALS:has_operator
        a             owl:ObjectProperty ;
        rdfs:comment  " the operator to apply\n@creationTimestamp 2016.02.08 at 15:03:36 EST" , " The operator in the [left OPERATOR right] tuple\n@creationTimestamp 2016.02.08 at 15:02:51 EST" ;
        rdfs:domain   IMMoRTALS_resources_constraints:ExpressionUnary , IMMoRTALS_resources_constraints:ExpressionBinary ;
        rdfs:range    IMMoRTALS_resources_constraints:Operator .

IMMoRTALS:has_selectionOptions
        a             owl:ObjectProperty ;
        rdfs:comment  " The DFUs to select between\n@creationTimestamp 2016.02.08 at 14:51:08 EST" ;
        rdfs:domain   IMMoRTALS_dfu:DfuSelectionMechanismActive ;
        rdfs:range    IMMoRTALS_dfu:DfuArray .

IMMoRTALS_functionality_datatype:PhysicalLocationExtent
        a             owl:Class ;
        rdfs:comment  " Representation of a location extent \n@author jstaples\n@creationTimestamp 2016.02.08 at 14:55:15 EST" .

IMMoRTALS:hasBytecodeArtifactElement
        a            owl:ObjectProperty ;
        rdfs:domain  IMMoRTALS_bytecode:BytecodeArtifactArray ;
        rdfs:range   IMMoRTALS_bytecode:BytecodeArtifact .

IMMoRTALS:has_methodName
        a             owl:ObjectProperty ;
        rdfs:comment  " The name of the method. Together with the method signature, forms a uniquely identifying tuple for the method in this class\n@creationTimestamp 2016.02.08 at 14:42:29 EST" ;
        rdfs:domain   IMMoRTALS_bytecode:AMethod ;
        rdfs:range    xsd:string .

IMMoRTALS:hasNetworkInterfaceElement
        a            owl:ObjectProperty ;
        rdfs:domain  IMMoRTALS_resources_network:NetworkInterfaceArray ;
        rdfs:range   IMMoRTALS_resources_network:NetworkInterface .

IMMoRTALS_resources_constraints_OperatorType:LESS_THAN
        a       IMMoRTALS_resources_constraints:OperatorType , owl:Class .

IMMoRTALS_resources_constraints:ExpressionBinary
        a                owl:Class ;
        rdfs:comment     " An expression of the form [left OPERATOR right] \n@author jstaples\n@creationTimestamp 2016.02.08 at 15:02:51 EST" ;
        rdfs:subClassOf  IMMoRTALS_resources_constraints:Expression .

IMMoRTALS_condition:CellularConnectionUnavailable
        a                owl:Class ;
        rdfs:comment     " The quality of the cellular data link on a platform \n@author jstaples\n@creationTimestamp 2016.02.08 at 14:44:13 EST" ;
        rdfs:subClassOf  IMMoRTALS_condition:NetworkConnectionQuality .

IMMoRTALS_resources:ExecutionPlatform
        a                owl:Class ;
        rdfs:comment     " A platform on which execution can occur. The platform is a combination of physical (e.g., memory, cpu) and logical (e.g., OS version, system libraries) components. \n@author jstaples\n@creationTimestamp 2016.02.08 at 14:57:09 EST" ;
        rdfs:subClassOf  IMMoRTALS_resources:PlatformResource .

IMMoRTALS:has_functionalityBeingPerformed
        a             owl:ObjectProperty ;
        rdfs:comment  " The functionality performed by the DFU\n@creationTimestamp 2016.02.08 at 14:50:13 EST" ;
        rdfs:domain   IMMoRTALS_dfu:Dfu ;
        rdfs:range    IMMoRTALS_functionality:Functionality .

IMMoRTALS_resources_constraints_OperatorType:DIFFERENCE_OF
        a       IMMoRTALS_resources_constraints:OperatorType , owl:Class .

IMMoRTALS_condition:LibraryAvailable
        a                owl:Class ;
        rdfs:comment     " A condition where some library is available \n@author jstaples\n@creationTimestamp 2016.02.08 at 14:45:23 EST" ;
        rdfs:subClassOf  IMMoRTALS_condition:PlatformCondition .

IMMoRTALS:has_osType  a  owl:ObjectProperty ;
        rdfs:comment  " E.g., Android\n@creationTimestamp 2016.02.08 at 15:07:42 EST" ;
        rdfs:domain   IMMoRTALS_resources_logical:OperatingSystem ;
        rdfs:range    xsd:string .

IMMoRTALS:has_inputType
        a             owl:ObjectProperty ;
        rdfs:comment  " An input type, which may or may not be encoded\n@creationTimestamp 2016.02.08 at 14:51:35 EST" , " The input type, which is encoded\n@creationTimestamp 2016.02.08 at 14:50:38 EST" ;
        rdfs:domain   IMMoRTALS_dfu:Encoder , IMMoRTALS_dfu:Decoder ;
        rdfs:range    IMMoRTALS_functionality_datatype:DataType , IMMoRTALS_functionality_datatype:EncodedDataType .

IMMoRTALS_resources_constraints_OperatorType:GREATER_THAN
        a       IMMoRTALS_resources_constraints:OperatorType , owl:Class .

IMMoRTALS_resources_performance_ResourcePerformanceType:Nominal
        a       IMMoRTALS_resources_performance:ResourcePerformanceType , owl:Class .

IMMoRTALS:has_gps  a  owl:ObjectProperty ;
        rdfs:comment  " A model of the gps topology\n@creationTimestamp 2016.02.08 at 15:05:52 EST" ;
        rdfs:domain   IMMoRTALS_resources_environment:OperatingEnvironment ;
        rdfs:range    IMMoRTALS_resources_gps:GpsEnvironment .

IMMoRTALS_resources_constraints:ExpressionEnumerationValue
        a                owl:Class ;
        rdfs:comment     " An expression that contains a single variable \n@author jstaples\n@creationTimestamp 2016.02.08 at 15:03:12 EST" ;
        rdfs:subClassOf  IMMoRTALS_resources_constraints:Expression .

IMMoRTALS_resources_constraints:ExpressionUnary
        a                owl:Class ;
        rdfs:comment     " A binding of an operator to a single expression \n@author jstaples\n@creationTimestamp 2016.02.08 at 15:03:36 EST" ;
        rdfs:subClassOf  IMMoRTALS_resources_constraints:Expression .

IMMoRTALS_dfu:Dfu  a  owl:Class ;
        rdfs:comment  " An abstraction that binds what is being done to how it is implemented in bytecode \n@author jstaples\n@creationTimestamp 2016.02.08 at 14:50:13 EST" .

IMMoRTALS_bytecode:AFieldArray
        a                owl:Class ;
        rdfs:subClassOf  IMMoRTALS:Array .

IMMoRTALS_resources_constraints_OperatorType:IS_ONE_OF
        a       IMMoRTALS_resources_constraints:OperatorType , owl:Class .

IMMoRTALS_resources_network:PhysicalLayerAbstraction
        a             owl:Class ;
        rdfs:comment  " An abstraction of the OSI physical layer \n@author jstaples\n@creationTimestamp 2016.02.08 at 15:12:30 EST" .

IMMoRTALS_resources_memory_MemoryType:SDRAM
        a       IMMoRTALS_resources_memory:MemoryType , owl:Class .

IMMoRTALS_resources_compute:Cpu
        a                owl:Class ;
        rdfs:comment     " Simple abstraction of a general-purpose compute device \n@author jstaples\n@creationTimestamp 2016.02.08 at 15:02:10 EST" ;
        rdfs:subClassOf  IMMoRTALS_resources:ComputeResource .

IMMoRTALS:has_observationTimeEpochMillis
        a             owl:DatatypeProperty ;
        rdfs:comment  " The time the performance is observed\n@creationTimestamp 2016.02.08 at 15:13:05 EST" ;
        rdfs:domain   IMMoRTALS_resources_performance:ResourcePerformanceObserved ;
        rdfs:range    xsd:long .

IMMoRTALS_resources_environment:RealWorldResource
        a                owl:Class ;
        rdfs:comment     " A resource that exists in the real world (e.g., terrain) \n@author jstaples\n@creationTimestamp 2016.02.08 at 15:06:11 EST" ;
        rdfs:subClassOf  IMMoRTALS_core:Resource .

IMMoRTALS:has_cpus  a  owl:ObjectProperty ;
        rdfs:comment  " Processors available for general purpose computation\n@creationTimestamp 2016.02.08 at 14:57:09 EST" ;
        rdfs:domain   IMMoRTALS_resources:ExecutionPlatform ;
        rdfs:range    IMMoRTALS_resources_compute:CpuArray .

IMMoRTALS_resources_performance_ResourcePerformanceType:LowerThreshold
        a       IMMoRTALS_resources_performance:ResourcePerformanceType , owl:Class .

IMMoRTALS:has_innerClasses
        a             owl:ObjectProperty ;
        rdfs:comment  " inner classes\n@creationTimestamp 2016.02.08 at 14:40:04 EST" ;
        rdfs:domain   IMMoRTALS_bytecode:AClass ;
        rdfs:range    IMMoRTALS_bytecode:AClassArray .

IMMoRTALS_condition:LogicalCondition
        a                owl:Class ;
        rdfs:comment     " A condition that cannot be observed through physical means (e.g., something happens inside a network) \n@author jstaples\n@creationTimestamp 2016.02.08 at 14:45:38 EST" ;
        rdfs:subClassOf  IMMoRTALS_condition:ObservableCondition .

IMMoRTALS:has_selectionMechanism
        a             owl:ObjectProperty ;
        rdfs:comment  " A DFU that allows us to inject the current environmental conditions and will pick the best dfu on our behalf\n@creationTimestamp 2016.02.08 at 14:51:19 EST" , " A DFU that allows us to specify the dfu that should be used\n@creationTimestamp 2016.02.08 at 14:51:08 EST" ;
        rdfs:domain   IMMoRTALS_dfu:DfuSelectionMechanismPassive , IMMoRTALS_dfu:DfuSelectionMechanismActive ;
        rdfs:range    IMMoRTALS_dfu:Dfu .

IMMoRTALS:has_acquireState
        a             owl:ObjectProperty ;
        rdfs:comment  " A DFU that allows us to acquire state before context switching\n@creationTimestamp 2016.02.08 at 14:49:12 EST" ;
        rdfs:domain   IMMoRTALS_dfu:ContextSwitchingMechanism ;
        rdfs:range    IMMoRTALS_dfu:Dfu .

IMMoRTALS_functionality:ConvolutionOnDevice
        a                owl:Class ;
        rdfs:comment     "\n@creationTimestamp 2016.02.08 at 14:51:43 EST" ;
        rdfs:subClassOf  IMMoRTALS_functionality:Convolution .

IMMoRTALS_resources_environment:OperatingEnvironment
        a             owl:Class ;
        rdfs:comment  " A description of the environment in which software is executed \n@author jstaples\n@creationTimestamp 2016.02.08 at 15:05:52 EST" .

IMMoRTALS:has_internetLayer
        a             owl:ObjectProperty ;
        rdfs:comment  " Describes how messages will be routed between two arbitrary points in a network of connected nodes E.g., IPV6\n@creationTimestamp 2016.02.08 at 15:12:17 EST" ;
        rdfs:domain   IMMoRTALS_resources_network:NetworkStackAbstraction ;
        rdfs:range    IMMoRTALS_resources_network:NetworkLayerAbstraction .

IMMoRTALS:has_terrain
        a             owl:ObjectProperty ;
        rdfs:comment  " The terrain in the operating environment\n@creationTimestamp 2016.02.08 at 15:06:06 EST" ;
        rdfs:domain   IMMoRTALS_resources_environment:PhysicalOperatingEnvironment ;
        rdfs:range    IMMoRTALS_resources_gps:Terrain .

IMMoRTALS_resources:NetworkResource
        a                owl:Class ;
        rdfs:comment     " A resource in the network sense \n@author jstaples\n@creationTimestamp 2016.02.08 at 14:57:30 EST" ;
        rdfs:subClassOf  IMMoRTALS_resources:IOResource .

IMMoRTALS_functionality_datatype:PhysicalLocation
        a             owl:Class ;
        rdfs:comment  " Representation of a physical location \n@author jstaples\n@creationTimestamp 2016.02.08 at 14:55:02 EST" .

IMMoRTALS_resources_memory_MemoryType:Cache_L2
        a       IMMoRTALS_resources_memory:MemoryType , owl:Class .

IMMoRTALS_resources_logical:NativeLibrary
        a                owl:Class ;
        rdfs:comment     " A native library \n@author jstaples\n@creationTimestamp 2016.02.08 at 15:07:24 EST" ;
        rdfs:subClassOf  IMMoRTALS_resources_logical:LogicalResource .

IMMoRTALS_condition_ConditionSensitivityImpactType:Degrades
        a       IMMoRTALS_condition:ConditionSensitivityImpactType , owl:Class .

IMMoRTALS:hasOutputElement
        a            owl:ObjectProperty ;
        rdfs:domain  IMMoRTALS_functionality:OutputArray ;
        rdfs:range   IMMoRTALS_functionality:Output .

IMMoRTALS_condition:Wind
        a                owl:Class ;
        rdfs:comment     " Wind \n@author jstaples\n@creationTimestamp 2016.02.08 at 14:47:48 EST" ;
        rdfs:subClassOf  IMMoRTALS_condition:WeatherCondition .

IMMoRTALS_resources_constraints:Range
        a             owl:Class ;
        rdfs:comment  " A range expresion \n@author jstaples\n@creationTimestamp 2016.02.08 at 15:04:43 EST" .

IMMoRTALS_resources:ResourcePerformanceMetricInstance
        a             owl:Class ;
        rdfs:comment  " An instance of a measured metric \n@author jstaples\n@creationTimestamp 2016.02.08 at 14:58:23 EST" .

IMMoRTALS:has_numChannels
        a             owl:DatatypeProperty ;
        rdfs:comment  " # of satellites the GPS receiver can lock onto e.g., cheapo GPS receivers use 4 whereas military grade can use 6+\n@creationTimestamp 2016.02.08 at 15:06:57 EST" ;
        rdfs:domain   IMMoRTALS_resources_gps:GpsReceiver ;
        rdfs:range    xsd:int .

IMMoRTALS:has_versionTag
        a             owl:ObjectProperty ;
        rdfs:comment  " E.g., 6.0_Marshmallow\n@creationTimestamp 2016.02.08 at 15:07:42 EST" ;
        rdfs:domain   IMMoRTALS_resources_logical:OperatingSystem ;
        rdfs:range    xsd:string .

IMMoRTALS:hasAMethodElement
        a            owl:ObjectProperty ;
        rdfs:domain  IMMoRTALS_bytecode:AMethodArray ;
        rdfs:range   IMMoRTALS_bytecode:AMethod .

IMMoRTALS_dfu:DataTypeConverter
        a                owl:Class ;
        rdfs:comment     " A simple DFU that converts between types \n@author jstaples\n@creationTimestamp 2016.02.08 at 14:49:32 EST" ;
        rdfs:subClassOf  IMMoRTALS_dfu:Dfu .

IMMoRTALS_resources_constraints_OperatorType:EQUAL
        a       IMMoRTALS_resources_constraints:OperatorType , owl:Class .

IMMoRTALS_dfu:DfuCannedSelectable
        a                owl:Class ;
        rdfs:comment     " A DFU that contains some functionality and some set of child DFUs for performing that functionality. These are immutable after application startup. \n@author jstaples\n@creationTimestamp 2016.02.08 at 14:50:17 EST" ;
        rdfs:subClassOf  IMMoRTALS_dfu:Dfu .

IMMoRTALS:has_inputs  a  owl:ObjectProperty ;
        rdfs:comment  " The inputs provided to the functionality abstraction. These can be either explicit (arguments) or implicit (e.g., field accesses)\n@creationTimestamp 2016.02.08 at 14:52:31 EST" ;
        rdfs:domain   IMMoRTALS_functionality:Functionality ;
        rdfs:range    IMMoRTALS_functionality:InputArray .

IMMoRTALS_bytecode:BytecodeArtifactArray
        a                owl:Class ;
        rdfs:subClassOf  IMMoRTALS:Array .

IMMoRTALS_resources_constraints_OperatorType:FALSE
        a       IMMoRTALS_resources_constraints:OperatorType , owl:Class .

IMMoRTALS:has_linkLayer
        a             owl:ObjectProperty ;
        rdfs:comment  " Describes how two nodes connected by some medium will communicate E.g., IEEE 802.2\n@creationTimestamp 2016.02.08 at 15:12:17 EST" ;
        rdfs:domain   IMMoRTALS_resources_network:NetworkStackAbstraction ;
        rdfs:range    IMMoRTALS_resources_network:LinkLayerAbstraction .

IMMoRTALS:has_memoryModel
        a             owl:ObjectProperty ;
        rdfs:comment  " A model of the memory for this object\n@creationTimestamp 2016.02.08 at 15:02:10 EST" , " A model of the memory for this object\n@creationTimestamp 2016.02.08 at 14:58:00 EST" , " A model of the memory for this object\n@creationTimestamp 2016.02.08 at 14:59:07 EST" , " A model of the memory for this object\n@creationTimestamp 2016.02.08 at 14:58:37 EST" , " A model of the memory for this object\n@creationTimestamp 2016.02.08 at 14:56:25 EST" ;
        rdfs:domain   IMMoRTALS_resources:DiskResource , IMMoRTALS_resources:Partition , IMMoRTALS_resources_compute:Gpu , IMMoRTALS_resources:Volume , IMMoRTALS_resources_compute:Cpu ;
        rdfs:range    IMMoRTALS_resources_memory:MemoryResource .

IMMoRTALS_dfu:ContextSwitchingMechanism
        a             owl:Class ;
        rdfs:comment  " Describes how to context switch from one DFU to another \n@author jstaples\n@creationTimestamp 2016.02.08 at 14:49:12 EST" .

IMMoRTALS:has_numCoresLogical
        a             owl:DatatypeProperty ;
        rdfs:comment  " The number of cores that appear to be available for independent execution. E.g., hyperthreading can map multiple logical threads onto a single physical compute resource\n@creationTimestamp 2016.02.08 at 15:02:10 EST" ;
        rdfs:domain   IMMoRTALS_resources_compute:Cpu ;
        rdfs:range    xsd:int .

IMMoRTALS_condition_ConditionSensitivityImpactType:Improves
        a       IMMoRTALS_condition:ConditionSensitivityImpactType , owl:Class .

IMMoRTALS_resources_constraints:ResourceConstraintExpression
        a             owl:Class ;
        rdfs:comment  " An expression for a constraint on a resource \n@author jstaples\n@creationTimestamp 2016.02.08 at 15:05:12 EST" .

IMMoRTALS_functionality:InputArray
        a                owl:Class ;
        rdfs:subClassOf  IMMoRTALS:Array .

IMMoRTALS:has_numberOfVisibleSatellites
        a             owl:DatatypeProperty ;
        rdfs:comment  " The number of satellites assumed to be visible\n@creationTimestamp 2016.02.08 at 15:06:46 EST" ;
        rdfs:domain   IMMoRTALS_resources_gps:GpsEnvironment ;
        rdfs:range    xsd:int .

IMMoRTALS_dfu:DfuInjectionMechanism
        a             owl:Class ;
        rdfs:comment  " Describes a method we call to inject this dfu \n@author jstaples\n@creationTimestamp 2016.02.08 at 14:50:51 EST" .

IMMoRTALS:has_canWrite
        a             owl:DatatypeProperty ;
        rdfs:comment  " True iff we can write this device\n@creationTimestamp 2016.02.08 at 15:11:21 EST" ;
        rdfs:domain   IMMoRTALS_resources_memory:MemoryResource ;
        rdfs:range    xsd:boolean .

IMMoRTALS_resources_environment:SignalQuality
        a             owl:Class ;
        rdfs:comment  " The quality of a signal \n@author jstaples\n@creationTimestamp 2016.02.08 at 15:06:19 EST" .

IMMoRTALS_resources_performance:ResourcePerformanceAnticipated
        a                owl:Class ;
        rdfs:comment     " Describes the anticipated performance of a resource in terms of some metric \n@author jstaples\n@creationTimestamp 2016.02.08 at 15:13:10 EST" ;
        rdfs:subClassOf  IMMoRTALS_resources_performance:ResourcePerformance .

IMMoRTALS_core:SoftwareDeployment
        a                owl:Class ;
        rdfs:comment     " Binds a software and platform abstraction to create an executable abstraction \n@author jstaples\n@creationTimestamp 2016.02.08 at 14:48:42 EST" ;
        rdfs:subClassOf  IMMoRTALS_core:Resource .

IMMoRTALS_condition:NetworkCondition
        a                owl:Class ;
        rdfs:comment     " A condition in a network \n@author jstaples\n@creationTimestamp 2016.02.08 at 14:45:49 EST" ;
        rdfs:subClassOf  IMMoRTALS_condition:LogicalCondition .

IMMoRTALS:has_injectState
        a             owl:ObjectProperty ;
        rdfs:comment  " the state injection mechanism\n@creationTimestamp 2016.02.08 at 14:50:51 EST" ;
        rdfs:domain   IMMoRTALS_dfu:DfuInjectionMechanism ;
        rdfs:range    IMMoRTALS_dfu:Dfu .

IMMoRTALS:has_binaryForm
        a             owl:ObjectProperty ;
        rdfs:comment  " The binary form of the artifact. For a naked class, bytecode; for a JAR, a compressed archive of classes; etc.\n@creationTimestamp 2016.02.08 at 14:42:54 EST" ;
        rdfs:domain   IMMoRTALS_bytecode:BytecodeArtifact ;
        rdfs:range    xsd:base64Binary .

IMMoRTALS_dfu:Decoder
        a                owl:Class ;
        rdfs:comment     " A DFU that decodes a datatype \n@author jstaples\n@creationTimestamp 2016.02.08 at 14:50:38 EST" ;
        rdfs:subClassOf  IMMoRTALS_dfu:Dfu .

IMMoRTALS_functionality:Input
        a                owl:Class ;
        rdfs:comment     " Something that provides input to a DFU \n@author jstaples\n@creationTimestamp 2016.02.08 at 14:52:35 EST" ;
        rdfs:subClassOf  IMMoRTALS_functionality:DataFlowMechanism .

IMMoRTALS_resources_memory_MemoryType:DRAM
        a       IMMoRTALS_resources_memory:MemoryType , owl:Class .

IMMoRTALS:has_uuid  a  owl:ObjectProperty ;
        rdfs:comment  " A unique identifier for this object\n@creationTimestamp 2016.02.08 at 14:42:29 EST" , " A unique identifier for this object\n@creationTimestamp 2016.02.08 at 14:41:08 EST" , " A unique identifier for this object\n@creationTimestamp 2016.02.08 at 14:40:04 EST" ;
        rdfs:domain   IMMoRTALS_bytecode:AMethod , IMMoRTALS_bytecode:AField , IMMoRTALS_bytecode:AClass ;
        rdfs:range    IMMoRTALS_bytecode:Uuid .

IMMoRTALS:has_satelliteId
        a             owl:ObjectProperty ;
        rdfs:comment  " A unique identifier for a statellite\n@creationTimestamp 2016.02.08 at 15:07:10 EST" ;
        rdfs:domain   IMMoRTALS_resources_gps:GpsSatellite ;
        rdfs:range    xsd:string .

IMMoRTALS_resources_network:NetworkConnection
        a                owl:Class ;
        rdfs:comment     " A network connection links two devices via some communication medium \n@author jstaples\n@creationTimestamp 2016.02.08 at 15:11:46 EST" ;
        rdfs:subClassOf  IMMoRTALS_resources:IOResource .

IMMoRTALS_resources_constraints:ExpressionVariable
        a                owl:Class ;
        rdfs:comment     " An expression that contains a single variable \n@author jstaples\n@creationTimestamp 2016.02.08 at 15:03:51 EST" ;
        rdfs:subClassOf  IMMoRTALS_resources_constraints:Expression .

IMMoRTALS:has_library
        a             owl:ObjectProperty ;
        rdfs:comment  " The library that is not available\n@creationTimestamp 2016.02.08 at 14:45:34 EST" , " The library that is available\n@creationTimestamp 2016.02.08 at 14:45:23 EST" ;
        rdfs:domain   IMMoRTALS_condition:LibraryUnavailable , IMMoRTALS_condition:LibraryAvailable ;
        rdfs:range    IMMoRTALS_bytecode:Library .

IMMoRTALS:hasResourceConstraintVariableBindingElement
        a            owl:ObjectProperty ;
        rdfs:domain  IMMoRTALS_resources_constraints:ResourceConstraintVariableBindingArray ;
        rdfs:range   IMMoRTALS_resources_constraints:ResourceConstraintVariableBinding .

IMMoRTALS_functionality:LocationProviderGps
        a                owl:Class ;
        rdfs:comment     " Provides a location using GPS signal triangulation \n@author jstaples\n@creationTimestamp 2016.02.08 at 14:53:06 EST" ;
        rdfs:subClassOf  IMMoRTALS_functionality:LocationProvider .

IMMoRTALS_resources_environment:WirelessSpectrum
        a             owl:Class ;
        rdfs:comment  " A spectrum block \n@author jstaples\n@creationTimestamp 2016.02.08 at 15:06:33 EST" .

IMMoRTALS:has_rangeExpression
        a             owl:ObjectProperty ;
        rdfs:comment  " An expression describing the perturbation\n@creationTimestamp 2016.02.08 at 15:13:40 EST" , " The range expression\n@creationTimestamp 2016.02.08 at 15:04:43 EST" ;
        rdfs:domain   IMMoRTALS_resources_perturbation:ResourcePerturbation , IMMoRTALS_resources_constraints:Range ;
        rdfs:range    IMMoRTALS_resources_constraints:Expression .

IMMoRTALS:has_structures
        a             owl:ObjectProperty ;
        rdfs:comment  " Assumptions about nearby structures that may affect the GPS signal\n@creationTimestamp 2016.02.08 at 15:06:46 EST" , " The structures in the operating environment\n@creationTimestamp 2016.02.08 at 15:06:06 EST" ;
        rdfs:domain   IMMoRTALS_resources_gps:GpsEnvironment , IMMoRTALS_resources_environment:PhysicalOperatingEnvironment ;
        rdfs:range    IMMoRTALS_resources_gps:Structures .

IMMoRTALS_bytecode:AMethod
        a                owl:Class ;
        rdfs:comment     " A method in a class \n@author jstaples\n@creationTimestamp 2016.02.08 at 14:42:29 EST" ;
        rdfs:subClassOf  IMMoRTALS_bytecode:ClassStructure .

IMMoRTALS_resources_constraints:Operator
        a             owl:Class ;
        rdfs:comment  " An operator for an expression \n@author jstaples\n@creationTimestamp 2016.02.08 at 15:04:19 EST" .

IMMoRTALS:has_encoding
        a             owl:ObjectProperty ;
        rdfs:comment  " The encoding for the data type (e.g., base64)\n@creationTimestamp 2016.02.08 at 14:54:09 EST" ;
        rdfs:domain   IMMoRTALS_functionality_datatype:EncodedDataType ;
        rdfs:range    IMMoRTALS_functionality_datatype:Encoding .

IMMoRTALS_functionality:OutputArray
        a                owl:Class ;
        rdfs:subClassOf  IMMoRTALS:Array .

IMMoRTALS_condition:PhysicalCondition
        a                owl:Class ;
        rdfs:comment     " A condition in the real world \n@author jstaples\n@creationTimestamp 2016.02.08 at 14:46:43 EST" ;
        rdfs:subClassOf  IMMoRTALS_condition:ObservableCondition .

IMMoRTALS_dfu:DecisionPointDfu
        a                owl:Class ;
        rdfs:comment     " A DFU that decides which of various child DFUs to use to implement the specified functionality \n@author jstaples\n@creationTimestamp 2016.02.08 at 14:49:42 EST" ;
        rdfs:subClassOf  IMMoRTALS_dfu:Dfu .

IMMoRTALS_condition_ConditionSensitivityImpactType:Optimizes
        a       IMMoRTALS_condition:ConditionSensitivityImpactType , owl:Class .

IMMoRTALS_resources:PartitionArray
        a                owl:Class ;
        rdfs:subClassOf  IMMoRTALS:Array .

IMMoRTALS:has_minFrequency
        a             owl:DatatypeProperty ;
        rdfs:comment  " The lower bound of the spectrum block\n@creationTimestamp 2016.02.08 at 15:06:33 EST" ;
        rdfs:domain   IMMoRTALS_resources_environment:WirelessSpectrum ;
        rdfs:range    xsd:double .

IMMoRTALS:has_systemLibraries
        a             owl:ObjectProperty ;
        rdfs:comment  " Libraries made available by the OS\n@creationTimestamp 2016.02.08 at 15:07:42 EST" ;
        rdfs:domain   IMMoRTALS_resources_logical:OperatingSystem ;
        rdfs:range    IMMoRTALS_resources_logical:LogicalResourceArray .

IMMoRTALS:has_type  a  owl:ObjectProperty ;
        rdfs:comment  " The type of performance we're describing\n@creationTimestamp 2016.02.08 at 15:13:25 EST" , " The semantic type of the data being passed\n@creationTimestamp 2016.02.08 at 14:52:02 EST" ;
        rdfs:domain   IMMoRTALS_resources_performance:ResourcePerformanceParameter , IMMoRTALS_functionality:DataFlowMechanism ;
        rdfs:range    IMMoRTALS_resources_performance:ResourcePerformanceType , IMMoRTALS_functionality_datatype:DataType .

IMMoRTALS:has_operatorType
        a             owl:ObjectProperty ;
        rdfs:comment  " An enumeration of permitted operations, one of which is selected\n@creationTimestamp 2016.02.08 at 15:04:19 EST" ;
        rdfs:domain   IMMoRTALS_resources_constraints:Operator ;
        rdfs:range    IMMoRTALS_resources_constraints:OperatorType .

IMMoRTALS:has_metric  a  owl:ObjectProperty ;
        rdfs:comment  " The metric we are using to describe performance as\n@creationTimestamp 2016.02.08 at 15:13:25 EST" , " The resource's performance metric to which the sensitivity will bind\n@creationTimestamp 2016.02.08 at 14:44:38 EST" ;
        rdfs:domain   IMMoRTALS_resources_performance:ResourcePerformanceParameter , IMMoRTALS_condition:ConditionSensitivity ;
        rdfs:range    IMMoRTALS_resources:ResourcePerformanceMetric .

IMMoRTALS_resources_memory:MemoryResource
        a                owl:Class ;
        rdfs:comment     " Memory \n@author jstaples\n@creationTimestamp 2016.02.08 at 15:11:21 EST" ;
        rdfs:subClassOf  IMMoRTALS_resources:PlatformResource .

IMMoRTALS:has_partitionsSpanned
        a             owl:ObjectProperty ;
        rdfs:comment  " The partitions the volume spans\n@creationTimestamp 2016.02.08 at 14:58:37 EST" ;
        rdfs:domain   IMMoRTALS_resources:Volume ;
        rdfs:range    IMMoRTALS_resources:PartitionArray .

IMMoRTALS_resources_memory_MemoryType:Cache_L3
        a       IMMoRTALS_resources_memory:MemoryType , owl:Class .

IMMoRTALS:hasResourcePerturbationElement
        a            owl:ObjectProperty ;
        rdfs:domain  IMMoRTALS_resources_perturbation:ResourcePerturbationArray ;
        rdfs:range   IMMoRTALS_resources_perturbation:ResourcePerturbation .

IMMoRTALS:has_deviceMemory
        a             owl:ObjectProperty ;
        rdfs:comment  " The device's physical memory\n@creationTimestamp 2016.02.08 at 14:57:09 EST" ;
        rdfs:domain   IMMoRTALS_resources:ExecutionPlatform ;
        rdfs:range    IMMoRTALS_resources_memory:PhysicalMemoryResource .

IMMoRTALS_resources:PlatformResource
        a                owl:Class ;
        rdfs:comment     " A resource present on a specific platform E.g., a library (code dependency)       a platform architecture (embedded linux, windows, ...)       compute resources (CPU, GPU, ...)       an external resource accessed via IO (network, disk, ...) \n@author jstaples\n@creationTimestamp 2016.02.08 at 14:58:16 EST" ;
        rdfs:subClassOf  IMMoRTALS_core:Resource .

IMMoRTALS:has_state  a  owl:ObjectProperty ;
        rdfs:comment  " The state of the DFU that must be carried across a context switch\n@creationTimestamp 2016.02.08 at 14:49:12 EST" ;
        rdfs:domain   IMMoRTALS_dfu:ContextSwitchingMechanism ;
        rdfs:range    IMMoRTALS_functionality_datatype:DataType .

IMMoRTALS_resources_network:NetworkInterface
        a                owl:Class ;
        rdfs:comment     " A device for connecting to a network \n@author jstaples\n@creationTimestamp 2016.02.08 at 15:11:50 EST" ;
        rdfs:subClassOf  IMMoRTALS_resources:PlatformResource .

IMMoRTALS_resources_gps:GpsSatellite
        a             owl:Class ;
        rdfs:comment  " a satellite that provides a GPS signal \n@author jstaples\n@creationTimestamp 2016.02.08 at 15:07:10 EST" .

IMMoRTALS:has_left  a  owl:ObjectProperty ;
        rdfs:comment  " The left statement in the [left OPERATOR right] tuple\n@creationTimestamp 2016.02.08 at 15:02:51 EST" ;
        rdfs:domain   IMMoRTALS_resources_constraints:ExpressionBinary ;
        rdfs:range    IMMoRTALS_resources_constraints:Expression .

IMMoRTALS_resources_constraints_OperatorType:QUOTIENT_OF
        a       IMMoRTALS_resources_constraints:OperatorType , owl:Class .

IMMoRTALS_core:Resource
        a             owl:Class ;
        rdfs:comment  " A description of something upon which software might depend E.g., a library (code dependency)       a platform architecture (embedded linux, windows, ...)       compute resources (CPU, GPU, ...)       an external resource accessed via IO (network, disk, ...) \n@author jstaples\n@creationTimestamp 2016.02.08 at 14:48:13 EST" .

IMMoRTALS_resources_performance:ResourcePerformanceParameterArray
        a                owl:Class ;
        rdfs:subClassOf  IMMoRTALS:Array .

IMMoRTALS:has_gpus  a  owl:ObjectProperty ;
        rdfs:comment  " Processors available for graphics processing\n@creationTimestamp 2016.02.08 at 14:57:09 EST" ;
        rdfs:domain   IMMoRTALS_resources:ExecutionPlatform ;
        rdfs:range    IMMoRTALS_resources_compute:GpuArray .

IMMoRTALS_resources_compute:Gpu
        a                owl:Class ;
        rdfs:comment     " Simple abstraction of a specialized compute device for graphics processing. \n@author jstaples\n@creationTimestamp 2016.02.08 at 14:59:07 EST" ;
        rdfs:subClassOf  IMMoRTALS_resources:ComputeResource .

IMMoRTALS:has_anticipatedPerturbations
        a             owl:ObjectProperty ;
        rdfs:comment  " The resource and environmental perturbations under which our software is expected to remain functional. E.g., maybe our software is expected to remain functional if the device runs out of local storage.\n@creationTimestamp 2016.02.08 at 14:48:09 EST" ;
        rdfs:domain   IMMoRTALS_core:DeploymentModel ;
        rdfs:range    IMMoRTALS_resources_perturbation:ResourcePerturbationArray .

IMMoRTALS_functionality_datatype:Image
        a                owl:Class ;
        rdfs:comment     " A top-level abstraction of an image, which may be presented and encoded in a variety of ways \n@author jstaples\n@creationTimestamp 2016.02.08 at 14:54:54 EST" ;
        rdfs:subClassOf  IMMoRTALS_functionality_datatype:DataType .

IMMoRTALS_resources_constraints_OperatorType:SUM_OF
        a       IMMoRTALS_resources_constraints:OperatorType , owl:Class .

IMMoRTALS_functionality:Output
        a                owl:Class ;
        rdfs:comment     " The output of a DFU \n@author jstaples\n@creationTimestamp 2016.02.08 at 14:53:49 EST" ;
        rdfs:subClassOf  IMMoRTALS_functionality:DataFlowMechanism .

IMMoRTALS_resources_memory_MemoryType:PCM
        a       IMMoRTALS_resources_memory:MemoryType , owl:Class .

IMMoRTALS_resources_constraints_OperatorType:OR
        a       IMMoRTALS_resources_constraints:OperatorType , owl:Class .

IMMoRTALS_resources_performance_ResourcePerformanceType:UpperThreshold
        a       IMMoRTALS_resources_performance:ResourcePerformanceType , owl:Class .

IMMoRTALS_resources_gps:GpsReceiver
        a             owl:Class ;
        rdfs:comment  " Models a GPS receiver \n@author jstaples\n@creationTimestamp 2016.02.08 at 15:06:57 EST" .

IMMoRTALS_condition:ConditionSensitivity
        a             owl:Class ;
        rdfs:comment  " Specifies that a resource is sensitive to a condition. Further specifies the impact of observing that condition on the resource's performance in terms of some metric. \n@author jstaples\n@creationTimestamp 2016.02.08 at 14:44:38 EST" .

IMMoRTALS_dfu:DfuSelectionMechanismPassive
        a                owl:Class ;
        rdfs:comment     " Describes a dfu that selects the best of a set of DFUs that perform some functionality based on current conditions. We should periodically update this component with current observations. \n@author jstaples\n@creationTimestamp 2016.02.08 at 14:51:19 EST" ;
        rdfs:subClassOf  IMMoRTALS_dfu:DfuCannedSelectable .

IMMoRTALS:has_resource
        a             owl:ObjectProperty ;
        rdfs:comment  " The resource for which performance will be described\n@creationTimestamp 2016.02.08 at 15:12:46 EST" , " A resource variable to use in an expression\n@creationTimestamp 2016.02.08 at 15:03:51 EST" , " The resource to which the sensitivity will bind\n@creationTimestamp 2016.02.08 at 14:44:38 EST" ;
        rdfs:domain   IMMoRTALS_resources_performance:ResourcePerformance , IMMoRTALS_resources_constraints:ExpressionVariable , IMMoRTALS_condition:ConditionSensitivity ;
        rdfs:range    IMMoRTALS_core:Resource .

IMMoRTALS_resources_logical_OsType:Windows
        a       IMMoRTALS_resources_logical:OsType , owl:Class .

IMMoRTALS_resources_constraints:ResourceConstraint
        a             owl:Class ;
        rdfs:comment  " A constraint on a resource \n@author jstaples\n@creationTimestamp 2016.02.08 at 15:04:57 EST" .

IMMoRTALS_resources_constraints:ExpressionNumber
        a                owl:Class ;
        rdfs:comment     " An expression that contains a single variable \n@author jstaples\n@creationTimestamp 2016.02.08 at 15:03:22 EST" ;
        rdfs:subClassOf  IMMoRTALS_resources_constraints:Expression .

IMMoRTALS_resources_constraints:OperatorType
        a                owl:Class ;
        rdfs:comment     " An enumeration of permitted operations \n@author jstaples\n@creationTimestamp 2016.02.05 at 13:55:09 EST" ;
        rdfs:subClassOf  IMMoRTALS:Enumeration .

IMMoRTALS:hasResourceElement
        a            owl:ObjectProperty ;
        rdfs:domain  IMMoRTALS_core:ResourceArray ;
        rdfs:range   IMMoRTALS_core:Resource .

IMMoRTALS_core:ResourceArray
        a                owl:Class ;
        rdfs:subClassOf  IMMoRTALS:Array .

IMMoRTALS:has_fromDataType
        a             owl:ObjectProperty ;
        rdfs:comment  " The type to convert from\n@creationTimestamp 2016.02.08 at 14:49:32 EST" ;
        rdfs:domain   IMMoRTALS_dfu:DataTypeConverter ;
        rdfs:range    IMMoRTALS_functionality_datatype:DataType .

IMMoRTALS_java_lang:StringArray
        a                owl:Class ;
        rdfs:subClassOf  IMMoRTALS:Array .

IMMoRTALS_condition:ProtonFluxEvent
        a                owl:Class ;
        rdfs:comment     " I.e., a solar flare.  These can disable satellites \n@author jstaples\n@creationTimestamp 2016.02.08 at 14:46:59 EST" ;
        rdfs:subClassOf  IMMoRTALS_condition:AtmosphericCondition .

IMMoRTALS:has_disks  a  owl:ObjectProperty ;
        rdfs:comment  " The device's disk hardware\n@creationTimestamp 2016.02.08 at 14:57:09 EST" ;
        rdfs:domain   IMMoRTALS_resources:ExecutionPlatform ;
        rdfs:range    IMMoRTALS_resources:DiskResourceArray .

IMMoRTALS:has_osPartition
        a             owl:ObjectProperty ;
        rdfs:comment  " The device's disk storage\n@creationTimestamp 2016.02.08 at 15:07:42 EST" ;
        rdfs:domain   IMMoRTALS_resources_logical:OperatingSystem ;
        rdfs:range    IMMoRTALS_resources:PartitionedDiskResource .

IMMoRTALS_resources_network:TransportLayerAbstraction
        a             owl:Class ;
        rdfs:comment  " An abstraction of the OSI transport layer \n@author jstaples\n@creationTimestamp 2016.02.08 at 15:12:34 EST" .

IMMoRTALS_resources_memory:VirtualMemoryResource
        a                owl:Class ;
        rdfs:comment     " Virtual memory (i.e., the amount of memory an application thinks exists on the system) \n@author jstaples\n@creationTimestamp 2016.02.08 at 15:10:06 EST" ;
        rdfs:subClassOf  IMMoRTALS_resources_memory:MemoryResource .

IMMoRTALS:has_variable
        a             owl:ObjectProperty ;
        rdfs:comment  " The resource being perturbed\n@creationTimestamp 2016.02.08 at 15:13:40 EST" , " The variable over which the range is defined\n@creationTimestamp 2016.02.08 at 15:04:43 EST" ;
        rdfs:domain   IMMoRTALS_resources_perturbation:ResourcePerturbation , IMMoRTALS_resources_constraints:Range ;
        rdfs:range    IMMoRTALS_core:Resource .

IMMoRTALS:Array  a  owl:Class .

IMMoRTALS:has_maxFrequency
        a             owl:DatatypeProperty ;
        rdfs:comment  " The upper bound of the spectrum block\n@creationTimestamp 2016.02.08 at 15:06:33 EST" ;
        rdfs:domain   IMMoRTALS_resources_environment:WirelessSpectrum ;
        rdfs:range    xsd:double .

IMMoRTALS_functionality:Functionality
        a             owl:Class ;
        rdfs:comment  " A description of what a functional unit of software does (but not how it is done). If we know that two different pieces of code do essentially the same thing in a different way, the idea is that we can adapt our software by swapping between them. \n@author jstaples\n@creationTimestamp 2016.02.08 at 14:52:31 EST" .

IMMoRTALS_condition_ConditionSensitivityImpactType:Breaks
        a       IMMoRTALS_condition:ConditionSensitivityImpactType , owl:Class .

IMMoRTALS_resources_perturbation:ResourcePerturbation
        a             owl:Class ;
        rdfs:comment  " Describes a perturbation to a resource \n@author jstaples\n@creationTimestamp 2016.02.08 at 15:13:40 EST" .

IMMoRTALS:hasGpuElement
        a            owl:ObjectProperty ;
        rdfs:domain  IMMoRTALS_resources_compute:GpuArray ;
        rdfs:range   IMMoRTALS_resources_compute:Gpu .

IMMoRTALS:hasAFieldElement
        a            owl:ObjectProperty ;
        rdfs:domain  IMMoRTALS_bytecode:AFieldArray ;
        rdfs:range   IMMoRTALS_bytecode:AField .

IMMoRTALS_resources:ComputeResource
        a                owl:Class ;
        rdfs:comment     " A type of resource that performs computation E.g., FPGA, CPU, GPU \n@author jstaples\n@creationTimestamp 2016.02.08 at 14:55:44 EST" ;
        rdfs:subClassOf  IMMoRTALS_resources:PlatformResource .

IMMoRTALS:has_resourceDependencies
        a             owl:ObjectProperty ;
        rdfs:comment  " The resources upon which the DFU depends, if any\n@creationTimestamp 2016.02.08 at 14:50:13 EST" ;
        rdfs:domain   IMMoRTALS_dfu:Dfu ;
        rdfs:range    IMMoRTALS_core:ResourceArray .

IMMoRTALS:has_right  a  owl:ObjectProperty ;
        rdfs:comment  " The right statement in the [left OPERATOR right] tuple\n@creationTimestamp 2016.02.08 at 15:02:51 EST" ;
        rdfs:domain   IMMoRTALS_resources_constraints:ExpressionBinary ;
        rdfs:range    IMMoRTALS_resources_constraints:Expression .

IMMoRTALS:has_platform
        a             owl:ObjectProperty ;
        rdfs:comment  " The platform on which the software will execute\n@creationTimestamp 2016.02.08 at 14:48:42 EST" , " The platform to which the condition applies\n@creationTimestamp 2016.02.08 at 14:46:55 EST" ;
        rdfs:domain   IMMoRTALS_core:SoftwareDeployment , IMMoRTALS_condition:PlatformCondition ;
        rdfs:range    IMMoRTALS_resources:ExecutionPlatform , IMMoRTALS_resources:PlatformResource .

IMMoRTALS_resources_performance:ResourcePerformanceParameter
        a             owl:Class ;
        rdfs:comment  " Describes the performance we anticipate from a resource in terms of some metric \n@author jstaples\n@creationTimestamp 2016.02.08 at 15:13:25 EST" .

IMMoRTALS:has_actualValue
        a             owl:ObjectProperty ;
        rdfs:comment  " The actual value observed\n@creationTimestamp 2016.02.08 at 15:03:12 EST" ;
        rdfs:domain   IMMoRTALS_resources_constraints:ExpressionEnumerationValue ;
        rdfs:range    xsd:string .

IMMoRTALS_resources_memory_MemoryType:ROM
        a       IMMoRTALS_resources_memory:MemoryType , owl:Class .

IMMoRTALS_resources_memory_MemoryType:SRAM
        a       IMMoRTALS_resources_memory:MemoryType , owl:Class .

IMMoRTALS_dfu:DfuSelectionMechanismActive
        a                owl:Class ;
        rdfs:comment     " A dfu that allows us to specify which of several children that perform some functionality should actually be used to achieve that functionality. We should periodically monitor conditions and update this component with the best component to use. \n@author jstaples\n@creationTimestamp 2016.02.08 at 14:51:08 EST" ;
        rdfs:subClassOf  IMMoRTALS_dfu:DfuCannedSelectable .

IMMoRTALS_condition:WeatherCondition
        a                owl:Class ;
        rdfs:comment     " A weather condition \n@author jstaples\n@creationTimestamp 2016.02.08 at 14:47:30 EST" ;
        rdfs:subClassOf  IMMoRTALS_condition:AtmosphericCondition .

IMMoRTALS_resources:PartitionedDiskResource
        a                owl:Class ;
        rdfs:comment     " A partitioned disk resource is a physical disk that has been partitioned into logical segments \n@author jstaples\n@creationTimestamp 2016.02.08 at 14:58:12 EST" ;
        rdfs:subClassOf  IMMoRTALS_resources:IOResource .

IMMoRTALS:hasStringElement
        a            owl:ObjectProperty ;
        rdfs:domain  IMMoRTALS_java_lang:StringArray ;
        rdfs:range   xsd:string .

IMMoRTALS:has_numCoresPhysical
        a             owl:DatatypeProperty ;
        rdfs:comment  " The number of cores actually available for independent execution\n@creationTimestamp 2016.02.08 at 15:02:10 EST" ;
        rdfs:domain   IMMoRTALS_resources_compute:Cpu ;
        rdfs:range    xsd:int .

IMMoRTALS_functionality_datatype:Time
        a             owl:Class ;
        rdfs:comment  " Representation of a point in time \n@author jstaples\n@creationTimestamp 2016.02.08 at 14:55:27 EST" .

IMMoRTALS:has_maxAvailableBytes
        a             owl:DatatypeProperty ;
        rdfs:comment  " The space available for writing\n@creationTimestamp 2016.02.08 at 15:11:21 EST" ;
        rdfs:domain   IMMoRTALS_resources_memory:MemoryResource ;
        rdfs:range    xsd:long .

IMMoRTALS:has_owner  a  owl:ObjectProperty ;
        rdfs:comment  " The class containing this feature\n@creationTimestamp 2016.02.08 at 14:43:30 EST" ;
        rdfs:domain   IMMoRTALS_bytecode:ClassStructure ;
        rdfs:range    IMMoRTALS_bytecode:AClass .

IMMoRTALS_resources_logical:OperatingSystem
        a                owl:Class ;
        rdfs:comment     " Simple model of an operating system \n@author jstaples\n@creationTimestamp 2016.02.08 at 15:07:42 EST" ;
        rdfs:subClassOf  IMMoRTALS_resources_logical:LogicalResource .

IMMoRTALS_condition:ObservableConditionArray
        a                owl:Class ;
        rdfs:subClassOf  IMMoRTALS:Array .

IMMoRTALS_functionality:ConvolutionRemote
        a                owl:Class ;
        rdfs:comment     "\n@creationTimestamp 2016.02.08 at 14:51:47 EST" ;
        rdfs:subClassOf  IMMoRTALS_functionality:Convolution .

IMMoRTALS_condition:NetworkCongested
        a                owl:Class ;
        rdfs:comment     " A model of network congestion \n@author jstaples\n@creationTimestamp 2016.02.08 at 14:46:26 EST" ;
        rdfs:subClassOf  IMMoRTALS_condition:NetworkCondition .

IMMoRTALS_resources_constraints_OperatorType:TRUE
        a       IMMoRTALS_resources_constraints:OperatorType , owl:Class .

IMMoRTALS:has_toDataType
        a             owl:ObjectProperty ;
        rdfs:comment  " The type to convert to\n@creationTimestamp 2016.02.08 at 14:49:32 EST" ;
        rdfs:domain   IMMoRTALS_dfu:DataTypeConverter ;
        rdfs:range    IMMoRTALS_functionality_datatype:DataType .

IMMoRTALS_resources_compute:GpuArray
        a                owl:Class ;
        rdfs:subClassOf  IMMoRTALS:Array .

IMMoRTALS_resources_logical_OsType:Android
        a       IMMoRTALS_resources_logical:OsType , owl:Class .

IMMoRTALS_bytecode:ClassStructure
        a             owl:Class ;
        rdfs:comment  " Anything concrete a class might contain (e.g., a field). Note that this is a recursive definition because classes can contain nested classes \n@author jstaples\n@creationTimestamp 2016.02.08 at 14:43:30 EST" .

IMMoRTALS_dfu:Encoder
        a                owl:Class ;
        rdfs:comment     " A DFU that encodes a datatype \n@author jstaples\n@creationTimestamp 2016.02.08 at 14:51:35 EST" ;
        rdfs:subClassOf  IMMoRTALS_dfu:Dfu .

IMMoRTALS:has_fieldDesc
        a             owl:ObjectProperty ;
        rdfs:comment  " The type descriptor of the field. Along with the name, this is a uniquely identifying tuple for the field in its parent class\n@creationTimestamp 2016.02.08 at 14:41:08 EST" ;
        rdfs:domain   IMMoRTALS_bytecode:AField ;
        rdfs:range    xsd:string .

IMMoRTALS:has_os  a   owl:ObjectProperty ;
        rdfs:comment  " The operating system and any patches/versions\n@creationTimestamp 2016.02.08 at 14:57:09 EST" ;
        rdfs:domain   IMMoRTALS_resources:ExecutionPlatform ;
        rdfs:range    IMMoRTALS_resources_logical:OperatingSystem .

IMMoRTALS:has_outputType
        a             owl:ObjectProperty ;
        rdfs:comment  " An output type, which is encoded\n@creationTimestamp 2016.02.08 at 14:51:35 EST" , " The output type, which may or may not be encoded\n@creationTimestamp 2016.02.08 at 14:50:38 EST" ;
        rdfs:domain   IMMoRTALS_dfu:Encoder , IMMoRTALS_dfu:Decoder ;
        rdfs:range    IMMoRTALS_functionality_datatype:EncodedDataType , IMMoRTALS_functionality_datatype:DataType .

IMMoRTALS_bytecode:Library
        a             owl:Class ;
        rdfs:comment  " A library is a logical aggregation of compilation artifacts \n@author jstaples\n@creationTimestamp 2016.02.08 at 14:43:53 EST" .

IMMoRTALS:hasSoftwareDeploymentElement
        a            owl:ObjectProperty ;
        rdfs:domain  IMMoRTALS_core:SoftwareDeploymentArray ;
        rdfs:range   IMMoRTALS_core:SoftwareDeployment .

IMMoRTALS:has_transportLayer
        a             owl:ObjectProperty ;
        rdfs:comment  " Describes how messages will be reliably delivered in an environment where individual messages may be lost or corrupted. E.g., TCP, UPD\n@creationTimestamp 2016.02.08 at 15:12:17 EST" ;
        rdfs:domain   IMMoRTALS_resources_network:NetworkStackAbstraction ;
        rdfs:range    IMMoRTALS_resources_network:TransportLayerAbstraction .

IMMoRTALS:hasPartitionElement
        a            owl:ObjectProperty ;
        rdfs:domain  IMMoRTALS_resources:PartitionArray ;
        rdfs:range   IMMoRTALS_resources:Partition .

IMMoRTALS_condition:PlatformCondition
        a                owl:Class ;
        rdfs:comment     " A condition that occurs on a platform (e.g., battery dies) \n@author jstaples\n@creationTimestamp 2016.02.08 at 14:46:55 EST" ;
        rdfs:subClassOf  IMMoRTALS_condition:LogicalCondition .

IMMoRTALS:hasDiskResourceElement
        a            owl:ObjectProperty ;
        rdfs:domain  IMMoRTALS_resources:DiskResourceArray ;
        rdfs:range   IMMoRTALS_resources:DiskResource .

IMMoRTALS_resources_constraints_OperatorType:EQUAL_LOGICAL
        a       IMMoRTALS_resources_constraints:OperatorType , owl:Class .

IMMoRTALS_resources_network:NetworkInterfaceArray
        a                owl:Class ;
        rdfs:subClassOf  IMMoRTALS:Array .

IMMoRTALS:hasLogicalResourceElement
        a            owl:ObjectProperty ;
        rdfs:domain  IMMoRTALS_resources_logical:LogicalResourceArray ;
        rdfs:range   IMMoRTALS_resources_logical:LogicalResource .

IMMoRTALS:has_triggeredConditions
        a             owl:ObjectProperty ;
        rdfs:comment  " One condition may trigger another\n@creationTimestamp 2016.02.08 at 14:44:38 EST" ;
        rdfs:domain   IMMoRTALS_condition:ConditionSensitivity ;
        rdfs:range    IMMoRTALS_condition:ObservableConditionArray .

IMMoRTALS_bytecode:AMethodArray
        a                owl:Class ;
        rdfs:subClassOf  IMMoRTALS:Array .

IMMoRTALS:has_uniqueIdentifier
        a             owl:ObjectProperty ;
        rdfs:comment  " The unique identifier\n@creationTimestamp 2016.02.08 at 15:20:20 EST" ;
        rdfs:domain   IMMoRTALS_bytecode:Uuid ;
        rdfs:range    xsd:string .

IMMoRTALS:has_classes
        a             owl:ObjectProperty ;
        rdfs:comment  " The classes contained in this artifact\n@creationTimestamp 2016.02.08 at 14:42:54 EST" ;
        rdfs:domain   IMMoRTALS_bytecode:BytecodeArtifact ;
        rdfs:range    IMMoRTALS_bytecode:AClassArray .

IMMoRTALS:has_hasFineGrainedEncryptedLocation
        a             owl:DatatypeProperty ;
        rdfs:comment  " true iff this satellite provides fine-grained location services to compatible military hardware\n@creationTimestamp 2016.02.08 at 15:07:10 EST" ;
        rdfs:domain   IMMoRTALS_resources_gps:GpsSatellite ;
        rdfs:range    xsd:boolean .

IMMoRTALS_resources_constraints_OperatorType:AND
        a       IMMoRTALS_resources_constraints:OperatorType , owl:Class .

IMMoRTALS_core:DeploymentModel
        a             owl:Class ;
        rdfs:comment  " Describes the deployment of one or more software products to one or more devices in an environment \n@author jstaples\n@creationTimestamp 2016.02.08 at 14:48:09 EST" .

IMMoRTALS_condition:NetworkConnectionQuality
        a                owl:Class ;
        rdfs:comment     " The quality of the cellular data link on a platform \n@author jstaples\n@creationTimestamp 2016.02.08 at 14:46:31 EST" ;
        rdfs:subClassOf  IMMoRTALS_condition:PlatformCondition .

IMMoRTALS_resources_performance:ResourcePerformanceObserved
        a                owl:Class ;
        rdfs:comment     " Describes the observed performance of a resource in terms of some metric \n@author jstaples\n@creationTimestamp 2016.02.08 at 15:13:05 EST" ;
        rdfs:subClassOf  IMMoRTALS_resources_performance:ResourcePerformance .

IMMoRTALS:has_softwareDeployments
        a             owl:ObjectProperty ;
        rdfs:comment  " The mappings of software to be deployed to the platforms on which the software will execute.\n@creationTimestamp 2016.02.08 at 14:48:09 EST" ;
        rdfs:domain   IMMoRTALS_core:DeploymentModel ;
        rdfs:range    IMMoRTALS_core:SoftwareDeploymentArray .

IMMoRTALS:has_operatingEnvironment
        a             owl:ObjectProperty ;
        rdfs:comment  " Describes the environment external to the platforms on which software will be run. The environment will likely change after deployment and is difficult to predict.\n@creationTimestamp 2016.02.08 at 14:48:09 EST" ;
        rdfs:domain   IMMoRTALS_core:DeploymentModel ;
        rdfs:range    IMMoRTALS_resources_environment:OperatingEnvironment .

IMMoRTALS:hasDfuElement
        a            owl:ObjectProperty ;
        rdfs:domain  IMMoRTALS_dfu:DfuArray ;
        rdfs:range   IMMoRTALS_dfu:Dfu .

IMMoRTALS_functionality:LocationProviderNetwork
        a                owl:Class ;
        rdfs:comment     " A coarse-grained location retrieval strategy based on network connectivity \n@author jstaples\n@creationTimestamp 2016.02.08 at 14:53:44 EST" ;
        rdfs:subClassOf  IMMoRTALS_functionality:LocationProvider .

IMMoRTALS:has_methods
        a             owl:ObjectProperty ;
        rdfs:comment  " methods belonging to this class\n@creationTimestamp 2016.02.08 at 14:40:04 EST" ;
        rdfs:domain   IMMoRTALS_bytecode:AClass ;
        rdfs:range    IMMoRTALS_bytecode:AMethodArray .

IMMoRTALS_condition_ConditionSensitivityImpactType:DegradesSignificantly
        a       IMMoRTALS_condition:ConditionSensitivityImpactType , owl:Class .

IMMoRTALS_resources:DiskResource
        a                owl:Class ;
        rdfs:comment     " A disk-based resource. Note that this may include non-disk devices that follow the disk storage paradigm. \n@author jstaples\n@creationTimestamp 2016.02.08 at 14:56:25 EST" ;
        rdfs:subClassOf  IMMoRTALS_resources:IOResource .

IMMoRTALS_resources_network:ApplicationLayerAbstraction
        a             owl:Class ;
        rdfs:comment  " An abstraction of the OSI application layer \n@author jstaples\n@creationTimestamp 2016.02.08 at 15:11:27 EST" .

IMMoRTALS:has_fileSystem
        a             owl:ObjectProperty ;
        rdfs:comment  " The OS's file system\n@creationTimestamp 2016.02.08 at 15:07:42 EST" ;
        rdfs:domain   IMMoRTALS_resources_logical:OperatingSystem ;
        rdfs:range    IMMoRTALS_resources:FileSystemResource .

IMMoRTALS_dfu:DfuArray
        a                owl:Class ;
        rdfs:subClassOf  IMMoRTALS:Array .

IMMoRTALS_bytecode:AClassArray
        a                owl:Class ;
        rdfs:subClassOf  IMMoRTALS:Array .

IMMoRTALS_resources_constraints_OperatorType:NEGATE_LOGICAL
        a       IMMoRTALS_resources_constraints:OperatorType , owl:Class .

IMMoRTALS:has_fields  a  owl:ObjectProperty ;
        rdfs:comment  " fields belonging to this class\n@creationTimestamp 2016.02.08 at 14:40:04 EST" ;
        rdfs:domain   IMMoRTALS_bytecode:AClass ;
        rdfs:range    IMMoRTALS_bytecode:AFieldArray .

IMMoRTALS:has_memoryType
        a             owl:ObjectProperty ;
        rdfs:comment  " The kind of memory this is\n@creationTimestamp 2016.02.08 at 15:11:13 EST" ;
        rdfs:domain   IMMoRTALS_resources_memory:PhysicalMemoryResource ;
        rdfs:range    IMMoRTALS_resources_memory:MemoryType .

IMMoRTALS_resources_memory:MemoryType
        a                owl:Class ;
        rdfs:comment     " Enumeration of various memory types \n@author jstaples\n@creationTimestamp 2016.02.08 at 15:09:55 EST" ;
        rdfs:subClassOf  IMMoRTALS:Enumeration .

IMMoRTALS:has_contextSwitchingMechanism
        a             owl:ObjectProperty ;
        rdfs:comment  " How do we swap between this and some other DFU?\n@creationTimestamp 2016.02.08 at 14:50:28 EST" , " How do we swap between this and some other DFU?\n@creationTimestamp 2016.02.08 at 14:49:42 EST" ;
        rdfs:domain   IMMoRTALS_dfu:DfuContextSwitchable , IMMoRTALS_dfu:DecisionPointDfu ;
        rdfs:range    IMMoRTALS_dfu:ContextSwitchingMechanism .

IMMoRTALS_resources_constraints_OperatorType:LESS_THAN_OR_EQUAL
        a       IMMoRTALS_resources_constraints:OperatorType , owl:Class .

IMMoRTALS:has_remoteDevice
        a             owl:ObjectProperty ;
        rdfs:comment  " The remote device\n@creationTimestamp 2016.02.08 at 15:11:46 EST" ;
        rdfs:domain   IMMoRTALS_resources_network:NetworkConnection ;
        rdfs:range    IMMoRTALS_resources:ExecutionPlatform .

IMMoRTALS:hasObservableConditionElement
        a            owl:ObjectProperty ;
        rdfs:domain  IMMoRTALS_condition:ObservableConditionArray ;
        rdfs:range   IMMoRTALS_condition:ObservableCondition .

IMMoRTALS_resources_logical:OsType
        a                owl:Class ;
        rdfs:comment     " The type of operating system \n@author jstaples\n@creationTimestamp 2016.02.05 at 14:17:03 EST" ;
        rdfs:subClassOf  IMMoRTALS:Enumeration .

IMMoRTALS_resources:ResourcePerformanceMetric
        a             owl:Class ;
        rdfs:comment  " An instance of a metric for describing the performance of some metric \n@author jstaples\n@creationTimestamp 2016.02.08 at 14:58:19 EST" .

IMMoRTALS_condition:AtmosphericCondition
        a                owl:Class ;
        rdfs:comment     " A condition present in the atmosphere \n@author jstaples\n@creationTimestamp 2016.02.08 at 14:44:06 EST" ;
        rdfs:subClassOf  IMMoRTALS_condition:EnvironmentalCondition .

IMMoRTALS_functionality:DataFlowMechanism
        a             owl:Class ;
        rdfs:comment  " A mechanism by which a DFU reads and writes data \n@author jstaples\n@creationTimestamp 2016.02.08 at 14:52:02 EST" .

IMMoRTALS:has_bytecodeLinkage
        a             owl:ObjectProperty ;
        rdfs:comment  " The location in code where the functionality is performed\n@creationTimestamp 2016.02.08 at 14:50:13 EST" ;
        rdfs:domain   IMMoRTALS_dfu:Dfu ;
        rdfs:range    IMMoRTALS_bytecode:BytecodeArtifact .

IMMoRTALS_resources_network:NetworkLayerAbstraction
        a             owl:Class ;
        rdfs:comment  " An abstraction of the OSI network layer \n@author jstaples\n@creationTimestamp 2016.02.05 at 14:19:00 EST" .

IMMoRTALS:has_performanceDescription
        a             owl:ObjectProperty ;
        rdfs:comment  " A parameterization of the metrics for that resource\n@creationTimestamp 2016.02.08 at 15:12:46 EST" ;
        rdfs:domain   IMMoRTALS_resources_performance:ResourcePerformance ;
        rdfs:range    IMMoRTALS_resources_performance:ResourcePerformanceParameterArray .

IMMoRTALS_resources:Partition
        a                owl:Class ;
        rdfs:comment     " A logical organizational abstraction for disks \n@author jstaples\n@creationTimestamp 2016.02.08 at 14:58:00 EST" ;
        rdfs:subClassOf  IMMoRTALS_resources:DiskResource .

IMMoRTALS:has_terrainModel
        a             owl:ObjectProperty ;
        rdfs:comment  " Assumptions about terrain that may affect the GPS signal\n@creationTimestamp 2016.02.08 at 15:06:46 EST" ;
        rdfs:domain   IMMoRTALS_resources_gps:GpsEnvironment ;
        rdfs:range    IMMoRTALS_resources_gps:Terrain .

IMMoRTALS:has_network
        a             owl:ObjectProperty ;
        rdfs:comment  " The network over which communication occurs\n@creationTimestamp 2016.02.08 at 15:11:46 EST" , " A model of the network topology in the environment\n@creationTimestamp 2016.02.08 at 15:05:52 EST" ;
        rdfs:domain   IMMoRTALS_resources_network:NetworkConnection , IMMoRTALS_resources_environment:OperatingEnvironment ;
        rdfs:range    IMMoRTALS_resources_network:NetworkStackAbstraction , IMMoRTALS_resources_network:NetworkTopology .

IMMoRTALS:has_nextLevel
        a             owl:ObjectProperty ;
        rdfs:comment  " The next memory in the hierarchy, if one exists. E.g., if this node is L3 cache, the next level memory would be physical memory\n@creationTimestamp 2016.02.08 at 15:08:31 EST" ;
        rdfs:domain   IMMoRTALS_resources_memory:MemoryHierarchyComponent ;
        rdfs:range    IMMoRTALS_resources_memory:MemoryResource .

IMMoRTALS_bytecode:AField
        a             owl:Class ;
        rdfs:comment  " A field in a class \n@author jstaples\n@creationTimestamp 2016.02.08 at 14:41:08 EST" .

IMMoRTALS:has_impact  a  owl:ObjectProperty ;
        rdfs:comment  " Qualitative scale of the impact on the metric\n@creationTimestamp 2016.02.08 at 14:44:38 EST" ;
        rdfs:domain   IMMoRTALS_condition:ConditionSensitivity ;
        rdfs:range    IMMoRTALS_condition:ConditionSensitivityImpactType .

IMMoRTALS:has_variableName
        a             owl:ObjectProperty ;
        rdfs:comment  " The name of the variable\n@creationTimestamp 2016.02.08 at 15:05:26 EST" ;
        rdfs:domain   IMMoRTALS_resources_constraints:ResourceConstraintVariableBinding ;
        rdfs:range    xsd:string .

IMMoRTALS:has_methodDesc
        a             owl:ObjectProperty ;
        rdfs:comment  " The type descriptor (binary signature) of the method. Together with the method name, forms a uniquely identifying tuple for the method in this class\n@creationTimestamp 2016.02.08 at 14:42:29 EST" ;
        rdfs:domain   IMMoRTALS_bytecode:AMethod ;
        rdfs:range    xsd:string .

IMMoRTALS_resources_gps:Structures
        a                owl:Class ;
        rdfs:comment     " The structures in the environment \n@author jstaples\n@creationTimestamp 2016.02.08 at 15:07:14 EST" ;
        rdfs:subClassOf  IMMoRTALS_resources_environment:OperatingEnvironment .

IMMoRTALS_condition:ConditionSensitivityImpactType
        a                owl:Class ;
        rdfs:comment     " Describes the performance impact of a sensitivity on a resource's performance \n@author jstaples\n@creationTimestamp 2016.02.04 at 13:34:06 EST" ;
        rdfs:subClassOf  IMMoRTALS:Enumeration .

IMMoRTALS_resources_compute:CpuArray
        a                owl:Class ;
        rdfs:subClassOf  IMMoRTALS:Array .

IMMoRTALS_resources_memory:MemoryHierarchyComponent
        a                owl:Class ;
        rdfs:comment     " Memory is typically arranged in a hierarchy. E.g., CPU cache{L1, L2, L3}, physical memory, disk. \n@author jstaples\n@creationTimestamp 2016.02.08 at 15:08:31 EST" ;
        rdfs:subClassOf  IMMoRTALS_resources_memory:MemoryResource .

IMMoRTALS_functionality_datatype:DataType
        a             owl:Class ;
        rdfs:comment  " A semantic data type \n@author jstaples\n@creationTimestamp 2016.02.08 at 14:53:55 EST" .

IMMoRTALS_functionality:LocationProviderManual
        a                owl:Class ;
        rdfs:comment     " A manual means of providing a location \n@author jstaples\n@creationTimestamp 2016.02.08 at 14:53:19 EST" ;
        rdfs:subClassOf  IMMoRTALS_functionality:LocationProvider .

IMMoRTALS:has_condition
        a             owl:ObjectProperty ;
        rdfs:comment  " An observable real-world condition that impacts the metric for the indicated resource\n@creationTimestamp 2016.02.08 at 14:44:38 EST" ;
        rdfs:domain   IMMoRTALS_condition:ConditionSensitivity ;
        rdfs:range    IMMoRTALS_condition:ObservableCondition .

IMMoRTALS:hasNetworkConnectionElement
        a            owl:ObjectProperty ;
        rdfs:domain  IMMoRTALS_resources_network:NetworkConnectionArray ;
        rdfs:range   IMMoRTALS_resources_network:NetworkConnection .

IMMoRTALS_functionality:Convolution
        a                owl:Class ;
        rdfs:comment     "\n@creationTimestamp 2016.02.08 at 14:51:40 EST" ;
        rdfs:subClassOf  IMMoRTALS_functionality:Functionality .

IMMoRTALS:has_outputs
        a             owl:ObjectProperty ;
        rdfs:comment  " The outputs provided by the functionality abstraction. These can be either explicit (return value) or implicit (locations written)\n@creationTimestamp 2016.02.08 at 14:52:31 EST" ;
        rdfs:domain   IMMoRTALS_functionality:Functionality ;
        rdfs:range    IMMoRTALS_functionality:OutputArray .

IMMoRTALS_dfu:DfuContextSwitchable
        a                owl:Class ;
        rdfs:comment     " An abstraction that binds what is being done to how it is implemented in bytecode \n@author jstaples\n@creationTimestamp 2016.02.08 at 14:50:28 EST" ;
        rdfs:subClassOf  IMMoRTALS_dfu:Dfu .

IMMoRTALS_resources_environment:PhysicalOperatingEnvironment
        a             owl:Class ;
        rdfs:comment  " Models the physical aspects of a real-world operating environment \n@author jstaples\n@creationTimestamp 2016.02.08 at 15:06:06 EST" .

IMMoRTALS:hasResourcePerformanceParameterElement
        a            owl:ObjectProperty ;
        rdfs:domain  IMMoRTALS_resources_performance:ResourcePerformanceParameterArray ;
        rdfs:range   IMMoRTALS_resources_performance:ResourcePerformanceParameter .

IMMoRTALS_condition:ServerFailure
        a                owl:Class ;
        rdfs:comment     " A server failure \n@author jstaples\n@creationTimestamp 2016.02.08 at 14:47:15 EST" ;
        rdfs:subClassOf  IMMoRTALS_condition:NetworkCondition .

IMMoRTALS:has_software
        a             owl:ObjectProperty ;
        rdfs:comment  " A model of the software to be executed\n@creationTimestamp 2016.02.08 at 14:48:42 EST" ;
        rdfs:domain   IMMoRTALS_core:SoftwareDeployment ;
        rdfs:range    IMMoRTALS_core:SoftwareAnalysisModel .

IMMoRTALS_resources_logical:LogicalResource
        a                owl:Class ;
        rdfs:comment     " A logical resource \n@author jstaples\n@creationTimestamp 2016.02.08 at 15:07:21 EST" ;
        rdfs:subClassOf  IMMoRTALS_resources:PlatformResource .

IMMoRTALS_resources_logical:LogicalResourceArray
        a                owl:Class ;
        rdfs:subClassOf  IMMoRTALS:Array .

IMMoRTALS_functionality:LocationProvider
        a                owl:Class ;
        rdfs:comment     " Provides a location \n@author jstaples\n@creationTimestamp 2016.02.08 at 14:52:44 EST" ;
        rdfs:subClassOf  IMMoRTALS_functionality:Functionality .

IMMoRTALS_core:SoftwareDeploymentArray
        a                owl:Class ;
        rdfs:subClassOf  IMMoRTALS:Array .

IMMoRTALS:has_anticipatedEndTimeEpochMillis
        a             owl:DatatypeProperty ;
        rdfs:comment  " The time the indicated performance will end\n@creationTimestamp 2016.02.08 at 15:13:10 EST" ;
        rdfs:domain   IMMoRTALS_resources_performance:ResourcePerformanceAnticipated ;
        rdfs:range    xsd:long .

IMMoRTALS:Enumeration
        a       owl:Class .

IMMoRTALS_condition_ConditionSensitivityImpactType:ImprovesSignificantly
        a       IMMoRTALS_condition:ConditionSensitivityImpactType , owl:Class .

IMMoRTALS_resources:Volume
        a                owl:Class ;
        rdfs:comment     " A logical volume may span multiple partitions \n@author jstaples\n@creationTimestamp 2016.02.08 at 14:58:37 EST" ;
        rdfs:subClassOf  IMMoRTALS_resources:DiskResource .

IMMoRTALS_condition:EnvironmentalCondition
        a                owl:Class ;
        rdfs:comment     " A condition in the real world, but more specifically the environment \n@author jstaples\n@creationTimestamp 2016.02.08 at 14:45:05 EST" ;
        rdfs:subClassOf  IMMoRTALS_condition:PhysicalCondition .

IMMoRTALS:has_fieldName
        a             owl:ObjectProperty ;
        rdfs:comment  " The name of the field specified by the programmer. Along with the field descriptor, this is a uniquely identifying tuple for the field in its parent class\n@creationTimestamp 2016.02.08 at 14:41:08 EST" ;
        rdfs:domain   IMMoRTALS_bytecode:AField ;
        rdfs:range    xsd:string .

IMMoRTALS_resources:FileSystemResource
        a                owl:Class ;
        rdfs:comment     " A file system \n@author jstaples\n@creationTimestamp 2016.02.08 at 14:57:14 EST" ;
        rdfs:subClassOf  IMMoRTALS_resources:IOResource .

IMMoRTALS:has_possibleValues
        a             owl:ObjectProperty ;
        rdfs:comment  " The possible values that could have been observed\n@creationTimestamp 2016.02.08 at 15:03:12 EST" ;
        rdfs:domain   IMMoRTALS_resources_constraints:ExpressionEnumerationValue ;
        rdfs:range    IMMoRTALS_java_lang:StringArray .

IMMoRTALS_resources_constraints_OperatorType:PRODUCT_OF
        a       IMMoRTALS_resources_constraints:OperatorType , owl:Class .

IMMoRTALS_resources_constraints_OperatorType:NEGATE
        a       IMMoRTALS_resources_constraints:OperatorType , owl:Class .

IMMoRTALS_functionality_datatype:EncodedDataType
        a                owl:Class ;
        rdfs:comment     " An encoded data type \n@author jstaples\n@creationTimestamp 2016.02.08 at 14:54:09 EST" ;
        rdfs:subClassOf  IMMoRTALS_functionality_datatype:DataType .

IMMoRTALS:has_constraint
        a             owl:ObjectProperty ;
        rdfs:comment  " The constraint expression\n@creationTimestamp 2016.02.08 at 15:04:57 EST" ;
        rdfs:domain   IMMoRTALS_resources_constraints:ResourceConstraint ;
        rdfs:range    IMMoRTALS_resources_constraints:Expression .

IMMoRTALS:has_anticipatedStartTimeEpochMillis
        a             owl:DatatypeProperty ;
        rdfs:comment  " The time the indicated performance will begin\n@creationTimestamp 2016.02.08 at 15:13:10 EST" ;
        rdfs:domain   IMMoRTALS_resources_performance:ResourcePerformanceAnticipated ;
        rdfs:range    xsd:long .

IMMoRTALS_bytecode:BytecodeArtifact
        a             owl:Class ;
        rdfs:comment  " A bytecode compilation artifact \n@author jstaples\n@creationTimestamp 2016.02.08 at 14:42:54 EST" .

IMMoRTALS_resources_gps:GpsEnvironment
        a             owl:Class ;
        rdfs:comment  " Describes an environment in which a GPS receiver is expected to operate \n@author jstaples\n@creationTimestamp 2016.02.08 at 15:06:46 EST" .

IMMoRTALS:has_canRead
        a             owl:DatatypeProperty ;
        rdfs:comment  " True iff we can read this device\n@creationTimestamp 2016.02.08 at 15:11:21 EST" ;
        rdfs:domain   IMMoRTALS_resources_memory:MemoryResource ;
        rdfs:range    xsd:boolean .

IMMoRTALS_core:SoftwareAnalysisModel
        a             owl:Class ;
        rdfs:comment  " A Discrete Functional Unit (DFU) analysis model. This is derived by static analysis of a compiled application with help from programmer-provided source code annotations \n@author jstaples\n@creationTimestamp 2016.02.08 at 14:48:18 EST" .

IMMoRTALS:has_value  a  owl:ObjectProperty , owl:DatatypeProperty ;
        rdfs:comment  " The metric value describing performance\n@creationTimestamp 2016.02.08 at 15:13:25 EST" , " The value observed\n@creationTimestamp 2016.02.08 at 15:03:22 EST" ;
        rdfs:domain   IMMoRTALS_resources_performance:ResourcePerformanceParameter , IMMoRTALS_resources_constraints:ExpressionNumber ;
        rdfs:range    IMMoRTALS_resources:ResourcePerformanceMetricInstance , xsd:double .

IMMoRTALS_resources_network:NetworkTopology
        a                owl:Class ;
        rdfs:comment     " Models the connections available in the network \n@author jstaples\n@creationTimestamp 2016.02.08 at 15:12:27 EST" ;
        rdfs:subClassOf  IMMoRTALS_resources:PlatformResource .

IMMoRTALS:has_expression
        a             owl:ObjectProperty ;
        rdfs:comment  " Simple surface form expression\n@creationTimestamp 2016.02.08 at 15:05:12 EST" , " The expression to evaluate\n@creationTimestamp 2016.02.08 at 15:03:36 EST" ;
        rdfs:domain   IMMoRTALS_resources_constraints:ResourceConstraintExpression , IMMoRTALS_resources_constraints:ExpressionUnary ;
        rdfs:range    xsd:string , IMMoRTALS_resources_constraints:Expression .

IMMoRTALS_resources_network:LinkLayerAbstraction
        a             owl:Class ;
        rdfs:comment  " An abstraction of the OSI link layer \n@author jstaples\n@creationTimestamp 2016.02.08 at 15:11:30 EST" .

IMMoRTALS:has_artifacts
        a             owl:ObjectProperty ;
        rdfs:comment  " The artifacts in the library\n@creationTimestamp 2016.02.08 at 14:43:53 EST" ;
        rdfs:domain   IMMoRTALS_bytecode:Library ;
        rdfs:range    IMMoRTALS_bytecode:BytecodeArtifactArray .

IMMoRTALS_condition:ObservableCondition
        a             owl:Class ;
        rdfs:comment  " A condition in the real world \n@author jstaples\n@creationTimestamp 2016.02.08 at 14:46:39 EST" .

IMMoRTALS_resources_network:NetworkConnectionArray
        a                owl:Class ;
        rdfs:subClassOf  IMMoRTALS:Array .

IMMoRTALS:has_resourceVariableRepresents
        a             owl:ObjectProperty ;
        rdfs:comment  " The resource being constrained\n@creationTimestamp 2016.02.08 at 15:05:26 EST" ;
        rdfs:domain   IMMoRTALS_resources_constraints:ResourceConstraintVariableBinding ;
        rdfs:range    IMMoRTALS_resources:PlatformResource .

IMMoRTALS_resources_gps:Terrain
        a                owl:Class ;
        rdfs:comment     " The terrain in the environment \n@author jstaples\n@creationTimestamp 2016.02.08 at 15:07:18 EST" ;
        rdfs:subClassOf  IMMoRTALS_resources_environment:OperatingEnvironment .

IMMoRTALS:hasAClassElement
        a            owl:ObjectProperty ;
        rdfs:domain  IMMoRTALS_bytecode:AClassArray ;
        rdfs:range   IMMoRTALS_bytecode:AClass .

IMMoRTALS_resources_network:NetworkStackAbstraction
        a                owl:Class ;
        rdfs:comment     " Standard OSI model of a network stack \n@author jstaples\n@creationTimestamp 2016.02.08 at 15:12:17 EST" ;
        rdfs:subClassOf  IMMoRTALS_resources:NetworkResource .

IMMoRTALS_functionality_datatype:Encoding
        a             owl:Class ;
        rdfs:comment  " A semantic encoding type \n@author jstaples\n@creationTimestamp 2016.02.08 at 14:54:13 EST" .

IMMoRTALS_resources_memory:PhysicalMemoryResource
        a                owl:Class ;
        rdfs:comment     " The physical memory of a system. I.e., the actual installed memory hardware. \n@author jstaples\n@creationTimestamp 2016.02.08 at 15:11:13 EST" ;
        rdfs:subClassOf  IMMoRTALS_resources_memory:MemoryResource .

IMMoRTALS:has_platformLibraries
        a             owl:ObjectProperty ;
        rdfs:comment  " Libraries available on the platform\n@creationTimestamp 2016.02.08 at 14:57:09 EST" ;
        rdfs:domain   IMMoRTALS_resources:ExecutionPlatform ;
        rdfs:range    IMMoRTALS_resources_logical:LogicalResourceArray .

IMMoRTALS_bytecode:Uuid
        a             owl:Class ;
        rdfs:comment  " A universally unique identifier for something \n@author jstaples\n@creationTimestamp 2016.02.08 at 15:20:20 EST" .

IMMoRTALS:has_physicalLayer
        a             owl:ObjectProperty ;
        rdfs:comment  " Describes how data is physically transmitted over some medium E.g., USB, Ethernet\n@creationTimestamp 2016.02.08 at 15:12:17 EST" ;
        rdfs:domain   IMMoRTALS_resources_network:NetworkStackAbstraction ;
        rdfs:range    IMMoRTALS_resources_network:PhysicalLayerAbstraction .

IMMoRTALS_condition_ConditionSensitivityImpactType:DoesNotAffect
        a       IMMoRTALS_condition:ConditionSensitivityImpactType , owl:Class .

IMMoRTALS:has_bytecodeConstruct
        a             owl:ObjectProperty ;
        rdfs:comment  " The bytecode construct providing the dataflow mechanism E.g., could be a value on the stack, a field, etc.\n@creationTimestamp 2016.02.08 at 14:52:02 EST" ;
        rdfs:domain   IMMoRTALS_functionality:DataFlowMechanism ;
        rdfs:range    IMMoRTALS_bytecode:AClass .

IMMoRTALS_bytecode:JarArtifact
        a                owl:Class ;
        rdfs:comment     " A Java ARchive (JAR) artifact \n@author jstaples\n@creationTimestamp 2016.02.08 at 14:43:39 EST" ;
        rdfs:subClassOf  IMMoRTALS_bytecode:BytecodeArtifact .

IMMoRTALS:hasCpuElement
        a            owl:ObjectProperty ;
        rdfs:domain  IMMoRTALS_resources_compute:CpuArray ;
        rdfs:range   IMMoRTALS_resources_compute:Cpu .

IMMoRTALS_functionality_datatype:TimeRange
        a             owl:Class ;
        rdfs:comment  " Representation of a window of time \n@author jstaples\n@creationTimestamp 2016.02.08 at 14:55:37 EST" .

IMMoRTALS_condition:CellularConnectionAvailable
        a                owl:Class ;
        rdfs:comment     " The quality of the cellular data link on a platform \n@author jstaples\n@creationTimestamp 2016.02.08 at 14:44:10 EST" ;
        rdfs:subClassOf  IMMoRTALS_condition:NetworkConnectionQuality .

IMMoRTALS_resources_constraints_OperatorType:GREATER_THAN_OR_EQUAL
        a       IMMoRTALS_resources_constraints:OperatorType , owl:Class .

IMMoRTALS_resources_constraints:ResourceConstraintVariableBindingArray
        a                owl:Class ;
        rdfs:subClassOf  IMMoRTALS:Array .

IMMoRTALS_resources_constraints:ResourceConstraintVariableBinding
        a             owl:Class ;
        rdfs:comment  " A variable binding in a constraint expression \n@author jstaples\n@creationTimestamp 2016.02.08 at 15:05:26 EST" .

IMMoRTALS_resources_logical_OsType:Mac
        a       IMMoRTALS_resources_logical:OsType , owl:Class .

IMMoRTALS:has_injectionMechanism
        a             owl:ObjectProperty ;
        rdfs:comment  " How we can inject the DFU\n@creationTimestamp 2016.02.08 at 14:49:12 EST" ;
        rdfs:domain   IMMoRTALS_dfu:ContextSwitchingMechanism ;
        rdfs:range    IMMoRTALS_dfu:DfuInjectionMechanism .

IMMoRTALS_bytecode:AClass
        a                owl:Class ;
        rdfs:comment     " The class is the fundamental compilation unit of bytecode. This is a a logical representation of a class. E.g., classes contain fields, methods, annotations, etc. \n@author jstaples\n@creationTimestamp 2016.02.08 at 14:40:04 EST" ;
        rdfs:subClassOf  IMMoRTALS_bytecode:ClassStructure .

IMMoRTALS_resources_performance:ResourcePerformance
        a             owl:Class ;
        rdfs:comment  " Describes the performance of a resource in terms of metrics \n@author jstaples\n@creationTimestamp 2016.02.08 at 15:12:46 EST" .

IMMoRTALS_resources_constraints:Expression
        a             owl:Class ;
        rdfs:comment  " An expression \n@author jstaples\n@creationTimestamp 2016.02.08 at 15:02:25 EST" .

IMMoRTALS:has_variables
        a             owl:ObjectProperty ;
        rdfs:comment  " Bindings of variables to variables present in the surface form expression\n@creationTimestamp 2016.02.08 at 15:05:12 EST" ;
        rdfs:domain   IMMoRTALS_resources_constraints:ResourceConstraintExpression ;
        rdfs:range    IMMoRTALS_resources_constraints:ResourceConstraintVariableBindingArray .

IMMoRTALS:has_applicationLayer
        a             owl:ObjectProperty ;
        rdfs:comment  " Describes how applications will interpret the data E.g., HTTP, HTTPS\n@creationTimestamp 2016.02.08 at 15:12:17 EST" ;
        rdfs:domain   IMMoRTALS_resources_network:NetworkStackAbstraction ;
        rdfs:range    IMMoRTALS_resources_network:ApplicationLayerAbstraction .

IMMoRTALS:hasInputElement
        a            owl:ObjectProperty ;
        rdfs:domain  IMMoRTALS_functionality:InputArray ;
        rdfs:range   IMMoRTALS_functionality:Input .

IMMoRTALS_resources:IOResource
        a                owl:Class ;
        rdfs:comment     " A type of resource that affects software IO E.g., network, disk, file system More specialized: camera, GPS \n@author jstaples\n@creationTimestamp 2016.02.08 at 14:57:20 EST" ;
        rdfs:subClassOf  IMMoRTALS_resources:PlatformResource .

IMMoRTALS_resources:DiskResourceArray
        a                owl:Class ;
        rdfs:subClassOf  IMMoRTALS:Array .

IMMoRTALS:has_partitions
        a             owl:ObjectProperty ;
        rdfs:comment  " The partitions\n@creationTimestamp 2016.02.08 at 14:58:12 EST" ;
        rdfs:domain   IMMoRTALS_resources:PartitionedDiskResource ;
        rdfs:range    IMMoRTALS_resources:PartitionArray .

IMMoRTALS_resources_performance:ResourcePerformanceType
        a                owl:Class ;
        rdfs:comment     " Describes the performance we anticipate from a resource in terms of some metric \n@author jstaples\n@creationTimestamp 2016.02.04 at 14:05:03 EST" ;
        rdfs:subClassOf  IMMoRTALS:Enumeration .

IMMoRTALS_resources_memory_MemoryType:Cache_L1
        a       IMMoRTALS_resources_memory:MemoryType , owl:Class .

IMMoRTALS:has_networkInterfaces
        a             owl:ObjectProperty ;
        rdfs:comment  " The mechanisms by which the device can connect to a network\n@creationTimestamp 2016.02.08 at 14:57:09 EST" ;
        rdfs:domain   IMMoRTALS_resources:ExecutionPlatform ;
        rdfs:range    IMMoRTALS_resources_network:NetworkInterfaceArray .

IMMoRTALS_resources_perturbation:ResourcePerturbationArray
        a                owl:Class ;
        rdfs:subClassOf  IMMoRTALS:Array .

IMMoRTALS_resources_logical_OsType:Linux
        a       IMMoRTALS_resources_logical:OsType , owl:Class .

IMMoRTALS_condition:Rain
        a                owl:Class ;
        rdfs:comment     " A condition in the real world that may have an impact on the software \n@author jstaples\n@creationTimestamp 2016.02.08 at 14:47:02 EST" ;
        rdfs:subClassOf  IMMoRTALS_condition:WeatherCondition .

IMMoRTALS:has_connections
        a             owl:ObjectProperty ;
        rdfs:comment  " The network topology is simplified by assuming it can be viewed as a set of available connections, each with their own performance characteristics\n@creationTimestamp 2016.02.08 at 15:12:27 EST" ;
        rdfs:domain   IMMoRTALS_resources_network:NetworkTopology ;
        rdfs:range    IMMoRTALS_resources_network:NetworkConnectionArray .
